syncable' before changing to ts_updates

src/syncablep.lean
@@ -8,7 +8,7 @@ variables {n : ℕ} {σ : Type} {ι : Type} {τ : ι → Type} [decidable_eq ι]
 
 /-- syncable with the exception that no threads is allowed to store 
 or load in stores and loads respectively -/
-def syncable' (stores : list ι) (loads : list ι) (s : state n σ τ) (m : memory τ) : Prop :=
+def syncable' (stores : set ι) (loads : set ι) (s : state n σ τ) (m : memory τ) : Prop :=
 (∀i:ι,
     (∀ tid, i ∉ (s.threads.nth tid).stores ∧ m i = (s.threads.nth tid).global i) ∨
     (∃ tid, i ∈ (s.threads.nth tid).stores ∧ m i = (s.threads.nth tid).global i ∧
@@ -16,7 +16,7 @@ def syncable' (stores : list ι) (loads : list ι) (s : state n σ τ) (m : memo
 (∀ i tid, i ∈ stores → i ∉ (s.threads.nth tid).stores) ∧
 (∀ i tid, i ∈ loads → i ∉ (s.threads.nth tid).loads)
 
-example (s : state n σ τ) (m : memory τ) : syncable' [] [] s m ↔ state.syncable s m := begin
+example (s : state n σ τ) (m : memory τ) : syncable' ∅ ∅ s m ↔ state.syncable s m := begin
     unfold syncable',
     simp,
     refl,
